@prefix : <https://www.w3.org/ns/plead#> .
@prefix owl: <http://www.w3.org/2002/07/owl#> .
@prefix rdf: <http://www.w3.org/1999/02/22-rdf-syntax-ns#> .
@prefix xml: <http://www.w3.org/XML/1998/namespace> .
@prefix xsd: <http://www.w3.org/2001/XMLSchema#> .
@prefix rdfs: <http://www.w3.org/2000/01/rdf-schema#> .
@base <https://www.w3.org/ns/plead> .

<https://www.w3.org/ns/plead> rdf:type owl:Ontology ;
                               owl:versionIRI <https://www.w3.org/ns/plead> ;
                               rdfs:comment """Vocablary used by the Explanation tool in PLEAD

A visualised Image of Vocablary
![Plead](Plead.png)""" .

#################################################################
#    Annotation properties
#################################################################

###  http://www.w3.org/1999/02/22-rdf-syntax-ns#resource
rdf:resource rdf:type owl:AnnotationProperty .


###  http://www.w3.org/1999/02/22-rdf-syntax-ns#type
rdf:type rdf:type owl:AnnotationProperty .


#################################################################
#    Classes
#################################################################

###  https://www.w3.org/ns/plead#AcceptanceDecision
:AcceptanceDecision rdf:type owl:Class ;
                    rdfs:subClassOf :DecisionResult ;
                    rdfs:comment "A positive resolution reached after consideration." ;
                    rdfs:isDefinedBy : ;
                    rdfs:label "Acceptance Decision" .


###  https://www.w3.org/ns/plead#ActivityType
:ActivityType rdf:type owl:Class ;
              rdfs:comment """The type of process done to reach resolution reached after consideration.

This class is subclass to 
**prov:** 
            [prov:Activity](http://www.w3.org/ns/prov#Activity)"""@en ;
              rdfs:isDefinedBy : ;
              rdfs:label "Activity Type" .


###  https://www.w3.org/ns/plead#AmendingData
:AmendingData rdf:type owl:Class ;
              rdfs:subClassOf :DataActivity ;
              rdfs:comment "make changes to data in order to make it more accurate." ;
              rdfs:isDefinedBy : ;
              rdfs:label "Amending Data" .


###  https://www.w3.org/ns/plead#AutomatedDecision
:AutomatedDecision rdf:type owl:Class ;
                   rdfs:subClassOf :Decision ;
                   owl:disjointWith :HumanDecision ;
                   rdfs:comment "A resolution reached after an automated consideration." ;
                   rdfs:isDefinedBy : ;
                   rdfs:label "Automated Decision" .


###  https://www.w3.org/ns/plead#Data
:Data rdf:type owl:Class ;
      rdfs:comment """The data holded on data subject by the current organisation. 

This class is subclass to 
**prov:** 
            [prov:Entity](http://www.w3.org/ns/prov#Entity)

This class is equivalent to 
**gdpr:** 
       [Data](https://w3id.org/GDPRtEXT#Data)""" ;
      rdfs:isDefinedBy : ;
      rdfs:label "Data" .


###  https://www.w3.org/ns/plead#DataActivity
:DataActivity rdf:type owl:Class ;
              rdfs:comment """The type of processes that can by done on data.

This class is subclass to 
**prov:** 
            [prov:Activity](http://www.w3.org/ns/prov#Activity)""" ;
              rdfs:isDefinedBy : ;
              rdfs:label "Data Activity" .


###  https://www.w3.org/ns/plead#DataController
:DataController rdf:type owl:Class ;
                rdfs:comment """The organisation that controls personal data.

This class is subclass to 
**prov:** 
            [prov:Organization](http://www.w3.org/ns/prov#Organization)

This class is equivalent to 
**gdpr:** 
            [Controller](https://w3id.org/GDPRtEXT#Controller)""" ;
                rdfs:isDefinedBy : ;
                rdfs:label "Data Controller" .


###  https://www.w3.org/ns/plead#DataErasureRequest
:DataErasureRequest rdf:type owl:Class ;
                    rdfs:subClassOf :Requests ;
                    rdfs:comment "The request to remove data." ;
                    rdfs:isDefinedBy : ;
                    rdfs:label "Data Erasure Request" .


###  https://www.w3.org/ns/plead#DataObjectionRequest
:DataObjectionRequest rdf:type owl:Class ;
                      rdfs:subClassOf :Requests ;
                      rdfs:comment "The request to citing a reason against procedure" ;
                      rdfs:isDefinedBy : ;
                      rdfs:label "Data Objection Request" .


###  https://www.w3.org/ns/plead#DataRectificationRequest
:DataRectificationRequest rdf:type owl:Class ;
                          rdfs:subClassOf :Requests ;
                          rdfs:comment "The request to putting something right." ;
                          rdfs:isDefinedBy : ;
                          rdfs:label "Data Rectify Request" .


###  https://www.w3.org/ns/plead#DataRestrictionRequest
:DataRestrictionRequest rdf:type owl:Class ;
                        rdfs:subClassOf :Requests ;
                        rdfs:comment "The request of restricting the data acesss" ;
                        rdfs:isDefinedBy : ;
                        rdfs:label "Data Restrict Request" .


###  https://www.w3.org/ns/plead#DataReviewRequest
:DataReviewRequest rdf:type owl:Class ;
                   rdfs:subClassOf :Requests ;
                   rdfs:comment "The request to assessing a procedure formally with the intention of instituting change if necessary." ;
                   rdfs:isDefinedBy : ;
                   rdfs:label "Data Review Request" .


###  https://www.w3.org/ns/plead#DataSubject
:DataSubject rdf:type owl:Class ;
             rdfs:comment """The data subject is the person with data at the current organisation.

This class is subclass to 
**prov:** 
            [prov:Agent](http://www.w3.org/ns/prov#Agent)

This class is equivalent to 
**gdpr:** 
            [DataSubject](https://w3id.org/GDPRtEXT#DataSubject)""" ;
             rdfs:isDefinedBy : ;
             rdfs:label "Data Subject" .


###  https://www.w3.org/ns/plead#Decision
:Decision rdf:type owl:Class ;
          rdfs:comment """The type of process done to reach resolution reached after consideration.

This class is subclass to 
**prov:** 
            [prov:Entity](http://www.w3.org/ns/prov#Entity)""" ;
          rdfs:isDefinedBy : ;
          rdfs:label "Decision" .


###  https://www.w3.org/ns/plead#DecisionResult
:DecisionResult rdf:type owl:Class ;
                rdfs:comment """A resolution reached after consideration.

This class is subclass to 
**prov:** 
            [prov:Entity](http://www.w3.org/ns/prov#Entity)""" ;
                rdfs:isDefinedBy : ;
                rdfs:label "Decision Result" .


###  https://www.w3.org/ns/plead#ErasingData
:ErasingData rdf:type owl:Class ;
             rdfs:subClassOf :DataActivity ;
             rdfs:comment """The process of removing data attributes.

This class is equivalent to 
**gdpr:** 
            [EraseData](https://w3id.org/GDPRtEXT#EraseData)""" ;
             rdfs:isDefinedBy : ;
             rdfs:label "Erasing" .


###  https://www.w3.org/ns/plead#ExternalData
:ExternalData rdf:type owl:Class ;
              rdfs:subClassOf :Data ;
              rdfs:comment "Data belonging to a DataSubject and under the control of the DataController." ;
              rdfs:isDefinedBy : ;
              rdfs:label "External Data" .


###  https://www.w3.org/ns/plead#HumanDecision
:HumanDecision rdf:type owl:Class ;
               rdfs:subClassOf :Decision ;
               rdfs:comment "A resolution reached after a human consideration." ;
               rdfs:isDefinedBy : ;
               rdfs:label "Human Decision" .


###  https://www.w3.org/ns/plead#HumanLedActivity
:HumanLedActivity rdf:type owl:Class ;
                  rdfs:subClassOf :ActivityType ;
                  rdfs:comment "An activity that is done by intervention of human." ;
                  rdfs:isDefinedBy : ;
                  rdfs:label "Human Led Activity" .


###  https://www.w3.org/ns/plead#MachineLedActivity
:MachineLedActivity rdf:type owl:Class ;
                    rdfs:subClassOf :ActivityType ;
                    rdfs:comment """An activity that is done using an automated process.

This class is equivalent to 
**gdpr:** 
       [AutomatedProcessing](https://w3id.org/GDPRtEXT#AutomatedProcessing)""" ;
                    rdfs:isDefinedBy : ;
                    rdfs:label "Machine Led Activity" .


###  https://www.w3.org/ns/plead#ObjectingData
:ObjectingData rdf:type owl:Class ;
               rdfs:subClassOf :DataActivity ;
               rdfs:comment "Citing a reason against procedure." ;
               rdfs:isDefinedBy : ;
               rdfs:label "Objecting" .


###  https://www.w3.org/ns/plead#PrivacyNotice
:PrivacyNotice rdf:type owl:Class ;
               rdfs:comment """Document that tells you what to expect us to do with your personal information when you make contact with us or use one of our services.

This class is subclass to 
**prov:** 
            [prov:Entity](http://www.w3.org/ns/prov#Entity)""" ;
               rdfs:isDefinedBy : ;
               rdfs:label "Privacy Notice" .


###  https://www.w3.org/ns/plead#ProcessingData
:ProcessingData rdf:type owl:Class ;
                rdfs:subClassOf :DataActivity ;
                rdfs:comment "Dealing with data/request using an official procedure." ;
                rdfs:isDefinedBy : ;
                rdfs:label "Processing" .


###  https://www.w3.org/ns/plead#RectifyingData
:RectifyingData rdf:type owl:Class ;
                rdfs:subClassOf :DataActivity ;
                rdfs:comment """The process of update/fix data attributes.

This class is equivalent to 
**gdpr:** 
            [RectifyData](https://w3id.org/GDPRtEXT#RectifyData)""" ;
                rdfs:isDefinedBy : ;
                rdfs:label "Rectifying" .


###  https://www.w3.org/ns/plead#RejectionDecision
:RejectionDecision rdf:type owl:Class ;
                   rdfs:subClassOf :DecisionResult ;
                   rdfs:comment "A negative resolution reached after consideration." ;
                   rdfs:isDefinedBy : ;
                   rdfs:label "Rejection Decision" .


###  https://www.w3.org/ns/plead#Requests
:Requests rdf:type owl:Class ;
          rdfs:comment """A request for process on the data.

This class is subclass to 
**prov:** 
            [prov:Entity](http://www.w3.org/ns/prov#Entity)""" ;
          rdfs:isDefinedBy : ;
          rdfs:label "Requests" .


###  https://www.w3.org/ns/plead#RestrictingData
:RestrictingData rdf:type owl:Class ;
                 rdfs:subClassOf :DataActivity ;
                 rdfs:comment "The process of restricting the data acesss." ;
                 rdfs:isDefinedBy : ;
                 rdfs:label "Restricting" .


###  https://www.w3.org/ns/plead#RetentionPeriod
:RetentionPeriod rdf:type owl:Class ;
                 rdfs:comment """The amount of time the continued possession of the document.

This class is subclass to 
**prov:** 
            [prov:Entity](http://www.w3.org/ns/prov#Entity)""" ;
                 rdfs:isDefinedBy : ;
                 rdfs:label "Retention Period" .


###  https://www.w3.org/ns/plead#ReviewingData
:ReviewingData rdf:type owl:Class ;
               rdfs:subClassOf :DataActivity ;
               rdfs:comment "Assessing a procedure formally with the intention of instituting change if necessary." ;
               rdfs:isDefinedBy : ;
               rdfs:label "Reviewing" .


###  https://www.w3.org/ns/plead#SubjectData
:SubjectData rdf:type owl:Class ;
             rdfs:subClassOf :Data ;
             rdfs:comment "Data provided to a DataController from a third party (that is not the Data Subject)" ;
             rdfs:isDefinedBy : ;
             rdfs:label "Subject Data" .


###  Generated by the OWL API (version 5.1.14) https://github.com/owlcs/owlapi/
